ulib/FStar.Seq.fst
@@ -1,3 +1,4 @@
 module FStar.Seq
 include FStar.Seq.Base
+include FStar.Seq.Derived
 include FStar.Seq.Properties
